Add definition examples

theories/glogic_examples.v
@@ -1,19 +1,18 @@
 Require Export glogic.
-Export GLogic.
 
 Theorem example1 C l T B :
   [{ C ; l --> (∇ T, ~ B) ≡ ~ (∇ T, B) }].
 Proof.
   destruct (nom_in_supp B T) as [a Ha].
   constructor; constructor.
-  - apply (rl_nabL a); tm_simpl.
+  - apply (rl_nabL _ a); tm_simpl.
     { assumption. }
-    apply contrapositive. apply (rl_nabL a Ha).
-    apply rl_id2.
-  - apply (rl_nabR a); tm_simpl.
+    apply contrapositive.
+    apply (rl_nabL _ a Ha). apply rl_id2.
+  - apply (rl_nabR _ a); tm_simpl.
     { assumption. }
-    apply contrapositive. apply (rl_nabR a Ha).
-    apply rl_id2.
+    apply contrapositive.
+    apply (rl_nabR _ a Ha). apply rl_id2.
 Qed.
 
 Theorem example2 C l T b c :
@@ -21,20 +20,20 @@ Theorem example2 C l T b c :
 Proof.
   destruct (nom_in_supp <{ b \/ c }> T) as [n Hn].
   constructor; constructor.
-  - apply (rl_nabL n) > [easy|].
+  - apply (rl_nabL _ n) > [easy|].
     tm_simpl. apply rl_orL.
-    + apply rl_orR1. apply (rl_nabR n).
+    + apply rl_orR1. apply (rl_nabR _ n).
       * unfold in_supp in *. simpl in *. intuition.
       * apply rl_id2.
-    + apply rl_orR2. apply (rl_nabR n).
+    + apply rl_orR2. apply (rl_nabR _ n).
       * unfold in_supp in *. simpl in *. intuition.
       * apply rl_id2.
-  - apply (rl_nabR n) > [easy|].
+  - apply (rl_nabR _ n) > [easy|].
     tm_simpl. apply rl_orL.
-    + apply rl_orR1. apply (rl_nabL n).
+    + apply rl_orR1. apply (rl_nabL _ n).
       * unfold in_supp in *. simpl in *. intuition.
       * apply rl_id2.
-    + apply rl_orR2. apply (rl_nabL n).
+    + apply rl_orR2. apply (rl_nabL _ n).
       * unfold in_supp in *. simpl in *. intuition.
       * apply rl_id2.
 Qed.
@@ -56,3 +55,45 @@ Proof.
     + assert (m ≡ ∅) by set_solver.
       rewrite H2 in H1. inversion H1.
       *)
+
+Definition ex4_clause_f (l : list ty) n :=
+  match l, n with
+  | [], 0 => Some (def_ind, <{\: ty_prp, 0}>)
+  | _, _ => None
+  end.
+
+Theorem example4 C :
+  ({ ex4_clause_f; C; $({[gtm_prd [] 0]}) --> gtm_bot }).
+Proof.
+  assert ( {[gtm_prd [] 0]} ≡ (∅ +; foldl tm_app (gtm_prd [] 0) [] : tm_set)).
+  - simpl. symmetry. apply union_empty.
+  - rewrite H.
+   eapply (rl_iL _ _ _ _ _ _ gtm_bot).
+    + simpl. reflexivity.
+    + simpl. intros. has_type.
+    + simpl. rewrite <- union_empty. apply rl_id.
+      apply tm_equiv_id.
+      apply rtsc_lr. simpl.
+      apply step_conv. left.
+      constructor.
+    + simpl. apply rl_id2.
+  Qed.
+
+Definition ex5_clause_f (l : list ty) n :=
+  match l, n with
+  | [], 0 => Some (def_cin, <{\: ty_prp, 0}>)
+  | _, _ => None
+  end.
+
+Theorem example5 C :
+  ({ ex5_clause_f; C; ∅ --> $(gtm_prd [] 0) }).
+Proof.
+  change (gtm_prd [] 0) with (foldl tm_app (gtm_prd [] 0) []).
+  eapply (rl_ciR _ _ _ _ _ _ gtm_top); simpl.
+  - reflexivity.
+  - intros. has_type.
+  - rewrite <- union_empty. apply rl_id.
+    apply tm_equiv_id. apply rtsc_rl. simpl.
+    apply step_conv. left. constructor.
+  - constructor.
+Qed.
